Typing.v
@@ -1,0 +1,109 @@
+(* This file is part of the LLIR Semantics project. *)
+(* Licensing information is available in the LICENSE file. *)
+(* (C) 2020 Nandor Licker. All rights reserved. *)
+
+Require Import Coq.Lists.List.
+
+Require Import LLIR.State.
+Require Import LLIR.LLIR.
+Require Import LLIR.Maps.
+
+
+Definition type_env := PTrie.t ty.
+
+Definition ptr_ty := I64.
+
+
+
+Definition get_inst_def (i: inst): option (ty * reg) :=
+  match i with
+  | LLInvoke dst _ _ _ _ => dst
+
+  | LLArg dst _ _ => Some dst
+  | LLInt8 dst _ _ => Some (I8, dst)
+  | LLInt16 _ dst _ => Some (I16, dst)
+  | LLInt32 _ dst _ => Some (I32, dst)
+  | LLInt64 _ dst _ => Some (I64, dst)
+
+  | LLFrame _ dst _ => Some (ptr_ty, dst)
+  | LLGlobal _ dst _ => Some (ptr_ty, dst)
+
+  | LLLd dst _ _ => Some dst
+  | LLUndef dst _ => Some dst
+  | LLUnop dst _ _ _ => Some dst
+  | LLBinop dst _ _ _ _ => Some dst
+
+  | LLSt _ _ _ => None
+  | LLRet _ => None
+  | LLJcc _ _ _ => None
+  | LLJmp _ => None
+  end.
+
+Definition ty_env_inst (insts: inst_map): type_env :=
+  PTrie.fold
+    (fun env _ i => 
+      match get_inst_def i with
+      | Some (ty, dst) => PTrie.set env dst ty
+      | None => env
+      end)
+    insts PTrie.empty.
+
+Definition ty_env_phi (phis: phi_map): type_env :=
+  PTrie.fold
+    (fun env _ block =>
+      List.fold_left
+        (fun env p =>
+          match p with
+          | LLPhi (ty, dst) _ => PTrie.set env dst ty
+          end)
+        block env)
+    phis PTrie.empty.
+
+Definition ty_env (f: func): type_env :=
+  PTrie.union (ty_env_inst f.(fn_insts)) (ty_env_phi f.(fn_phis)).
+
+Definition well_typed_reg (env: type_env) (r: reg) (ty: ty) :=
+  env ! r = Some ty.
+
+(*
+Inductive well_typed_inst: type_env -> inst -> Prop := .
+  | typed_jmp:
+
+  | LLInvoke dst _ _ _ _ => dst
+
+  | LLArg dst _ _ => Some dst
+  | LLInt8 dst _ _ => Some (I8, dst)
+  | LLInt16 _ dst _ => Some (I16, dst)
+  | LLInt32 _ dst _ => Some (I32, dst)
+  | LLInt64 _ dst _ => Some (I64, dst)
+
+  | LLFrame _ dst _ => Some (ptr_ty, dst)
+  | LLGlobal _ dst _ => Some (ptr_ty, dst)
+
+  | LLLd dst _ _ => Some dst
+  | LLUndef dst _ => Some dst
+  | LLUnop dst _ _ _ => Some dst
+  | LLBinop dst _ _ _ _ => Some dst
+
+  | LLSt _ _ _ => None
+  | LLRet _ => None
+  | LLJcc _ _ _ => None
+  | LLJmp _ => None
+  *)
+Definition well_typed_insts (env: type_env) (insts: inst_map) := 
+  False.
+
+Inductive well_typed_phi: type_env -> phi -> Prop :=
+  | typed_phi:
+    forall (env: type_env) (p: phi),
+      well_typed_phi env p
+  .
+
+Definition well_typed_phis (env: type_env) (phis: phi_map) :=
+  False.
+
+Definition well_typed (f: func) :=
+  well_typed_insts (ty_env f) f.(fn_insts)
+  /\
+  well_typed_phis (ty_env f) f.(fn_phis).
+
